coq/Dispatch.v
@@ -1,0 +1,76 @@
+Require Import LibTactics.
+Require Import Coq.micromega.Lia.
+Require Import LN_Lemmas.
+Require Export SimpleSub.
+
+(* Two types are sim iff they are splu from a value type *)
+Lemma sim_no_distinguishability : forall A B,
+    sim A B -> Distinguishability A B -> False.
+Proof with solve_false.
+  introv Sim Dis.
+  induction Sim; intros.
+  - induction Dis; try inverts_typ...
+    + inverts H...
+    + inverts H1...
+  - forwards* : distinguishability_rcd_inv Dis.
+  - inverts Dis...
+  - inverts Dis...
+Qed.
+
+Lemma dispatch_gen : forall (A1 A2 B B' C1 C2' : typ),
+    Mergeability A1 A2 ->
+    ApplyTy A1 B C1 -> NApplyTy A1 B' -> ApplyTy A2 B' C2' ->
+    NApplyTy A2 B -> (* this premise is not on the paper def *)
+    Distinguishability B B'.
+Proof with elia; solve_false.
+  (* introv Val1 Val2 App1 PSub App2. *)
+  (* indTypSize (size_typ V + size_typ V' + size_typ A). *)
+  (* lets~ [Hu|(?&?&Hu)]: ordu_or_split V'. *)
+  (* lets~ [Hu'|(?&?&Hu')]: ordu_or_split V. *)
+Admitted.
+
+(* This is equivalent to the dispatch lemma w/o ordu constraints *)
+Lemma applyty_merge_sim : forall A A' B B' x1 x2,
+    Mergeability A A' -> sim B B' ->
+    ApplyTy A B x1 -> ApplyTy A' B' x2 ->
+    exists y, ApplyTy A' B y \/ ApplyTy A B' y.
+Proof with solve_false.
+  introv HM HS HA1 HA2.
+  forwards* [(?&?)|?]: applyty_total A B'.
+  forwards* [(?&?)|?]: applyty_total A' B.
+  false. applys sim_no_distinguishability HS.
+  applys* dispatch_gen HM.
+Qed.
+
+Lemma lemma_for_B16 : forall A A' V B1 B2 x1 x2,
+    Mergeability A A' -> isValTyp V
+    -> splu V B1 B2 -> ApplyTy A B1 x1 -> ApplyTy A' B2 x2 ->
+    exists y, ApplyTy A' B1 y \/ ApplyTy A B2 y.
+Proof.
+  intros. applys~ applyty_merge_sim.
+  - applys sim2similar.
+    unfold similar. exists*.
+  - eauto.
+  - eauto.
+Qed.
+
+(* B.16 Inversion of Abstract Application to Value Types *)
+(* Here we only consider V to be StackArg. Note that V can also be StackTypArg
+but that case is trivial *)
+Lemma applyty_valtyp_inter_inv : forall (A A' V B : typ),
+    ApplyTy (A&A') V B -> isValTyp V -> TypeWF nil (A&A') ->
+    exists B', ApplyTy A V B' \/ ApplyTy A' V B'.
+Proof with solve_false.
+  introv HA HV WF.
+  indTypSize (size_typ V).
+  lets~ [Hu|(?&?&Hu)]: ordu_or_split V.
+  - inverts HA... all: exists*.
+  - inverts_typ.
+    inverts* HA.
+    forwards~ (?&[?|?]): IH H3; elia; forwards~ (?&[?|?]): IH H5; elia.
+    1,4: exists*.
+    * inverts WF. forwards~ (?&[?|?]): lemma_for_B16 H2 H1 H4.
+      all: exists*.
+    * inverts WF. forwards~ (?&[?|?]): lemma_for_B16 H2 H1 H4.
+      all: exists*.
+Qed.
